Remove more admits

src/lcertify/Certify.v
@@ -87,34 +87,34 @@ Proof.
 Qed.
 
 
-Inductive sim_time (ts:Time.t) (mem1 mem2:Memory.t) (v1 v2:Time.t): Prop :=
+Inductive sim_time (ts:Time.t) (v1 v2:Time.t): Prop :=
 | sim_time_intro
     (TS: v2 <= ts -> v1 = v2)
 .
 Hint Constructors sim_time.
 
-Inductive sim_view (ts:Time.t) (mem1 mem2:Memory.t) (v1 v2:View.t (A:=unit)): Prop :=
+Inductive sim_view (ts:Time.t) (v1 v2:View.t (A:=unit)): Prop :=
 | sim_view_intro
     (TS: v2.(View.ts) <= ts -> v1 = v2)
 .
 Hint Constructors sim_view.
 
-Inductive sim_val (ts:Time.t) (mem1 mem2:Memory.t) (v1 v2:ValA.t (A:=View.t (A:=unit))): Prop :=
+Inductive sim_val (ts:Time.t) (v1 v2:ValA.t (A:=View.t (A:=unit))): Prop :=
 | sim_val_intro
     (TS: v2.(ValA.annot).(View.ts) <= ts -> v1 = v2)
 .
 Hint Constructors sim_val.
 
-Inductive sim_rmap (ts:Time.t) (mem1 mem2:Memory.t) (rmap1 rmap2:RMap.t (A:=View.t (A:=unit))): Prop :=
+Inductive sim_rmap (ts:Time.t) (rmap1 rmap2:RMap.t (A:=View.t (A:=unit))): Prop :=
 | sim_rmap_intro
-    (RMAP: IdMap.Forall2 (fun _ => sim_val ts mem1 mem2) rmap1 rmap2)
+    (RMAP: IdMap.Forall2 (fun _ => sim_val ts) rmap1 rmap2)
 .
 Hint Constructors sim_rmap.
 
-Inductive sim_state (ts:Time.t) (mem1 mem2:Memory.t) (st1 st2:State.t (A:=View.t (A:=unit))): Prop :=
+Inductive sim_state (ts:Time.t) (st1 st2:State.t (A:=View.t (A:=unit))): Prop :=
 | sim_state_intro
     (STMTS: st1.(State.stmts) = st2.(State.stmts))
-    (RMAP: sim_rmap ts mem1 mem2 st1.(State.rmap) st2.(State.rmap))
+    (RMAP: sim_rmap ts st1.(State.rmap) st2.(State.rmap))
 .
 Hint Constructors sim_state.
 
@@ -137,7 +137,6 @@ Inductive sim_fwdbank (ts:Time.t) (mem1 mem2:Memory.t) (loc:Loc.t) (fwd1 fwd2:Fw
     (ABOVE: ts < fwd2.(FwdItem.view).(View.ts))
     (LATEST: Memory.latest loc fwd1.(FwdItem.ts) (length mem1) mem1)
     (EX: fwd1.(FwdItem.ex) = fwd2.(FwdItem.ex))
-    (READ: Memory.read loc fwd1.(FwdItem.ts) mem1 = Memory.read loc fwd2.(FwdItem.ts) mem2)
 .
 
 (* TODO: move many lemmas *)
@@ -162,15 +161,15 @@ Lemma sim_fwd_view1 tid ts mem1 mem2 loc coh1 coh2 fwd1 fwd2 o
       (WF1: Local.wf_fwdbank loc mem1 coh1 fwd1)
       (WF2: Local.wf_fwdbank loc mem2 coh2 fwd2)
       (MEM: sim_mem tid ts mem1 mem2):
-  sim_view ts mem1 mem2 (FwdItem.read_view fwd1 fwd1.(FwdItem.ts) o) (FwdItem.read_view fwd2 fwd2.(FwdItem.ts) o).
+  sim_view ts (FwdItem.read_view fwd1 fwd1.(FwdItem.ts) o) (FwdItem.read_view fwd2 fwd2.(FwdItem.ts) o).
 Proof.
   destruct fwd1 as [ts1 view1 ex1].
   destruct fwd2 as [ts2 view2 ex2].
   unfold FwdItem.read_view. s. inv WF1. inv WF2. inv MEM.
   inv FWD; ss; repeat condtac; ss.
   all: repeat match goal with
-              | [H: sim_time _ _ _ _ _ |- _] => inv H
-              | [H: sim_view _ _ _ _ _ |- _] => inv H
+              | [H: sim_time _ _ _ |- _] => inv H
+              | [H: sim_view _ _ _ |- _] => inv H
               | [H: FwdItem.mk _ _ _ = FwdItem.mk _ _ _ |- _] => inv H
               end.
   all: unfold Time.t in *.
@@ -184,15 +183,15 @@ Lemma sim_fwd_view2 tid ts mem1 mem2 loc coh1 coh2 fwd1 fwd2 t o
       (WF2: Local.wf_fwdbank loc mem2 coh2 fwd2)
       (MEM: sim_mem tid ts mem1 mem2)
       (TS: fwd2.(FwdItem.ts) < t):
-  sim_view ts mem1 mem2 (FwdItem.read_view fwd1 t o) (FwdItem.read_view fwd2 t o).
+  sim_view ts (FwdItem.read_view fwd1 t o) (FwdItem.read_view fwd2 t o).
 Proof.
   destruct fwd1 as [ts1 view1 ex1].
   destruct fwd2 as [ts2 view2 ex2].
   unfold FwdItem.read_view. s. inv WF1. inv WF2. inv MEM.
   inv FWD; ss; repeat condtac; ss.
   all: repeat match goal with
-              | [H: sim_time _ _ _ _ _ |- _] => inv H
-              | [H: sim_view _ _ _ _ _ |- _] => inv H
+              | [H: sim_time _ _ _ |- _] => inv H
+              | [H: sim_view _ _ _ |- _] => inv H
               | [H: FwdItem.mk _ _ _ = FwdItem.mk _ _ _ |- _] => inv H
               end.
   all: unfold Time.t in *.
@@ -239,19 +238,19 @@ Inductive sim_exbank (tid:Id.t) (ts:Time.t) (mem1 mem2:Memory.t) (eb1 eb2:Exbank
            (BELOW: t <= ts)
            (EXCLUSIVE: Memory.exclusive tid eb2.(Exbank.loc) eb2.(Exbank.ts) t mem2),
         Memory.exclusive tid eb1.(Exbank.loc) eb1.(Exbank.ts) t mem1)
-    (EBVIEW: sim_view ts mem1 mem2 eb1.(Exbank.view) eb2.(Exbank.view))
+    (EBVIEW: sim_view ts eb1.(Exbank.view) eb2.(Exbank.view))
 .
 Hint Constructors sim_exbank.
 
 Inductive sim_lc (tid:Id.t) (ts:Time.t) (mem1 mem2:Memory.t) (lc1 lc2:Local.t (A:=unit)): Prop :=
 | sim_lc_intro
-    (COH: forall loc, sim_view ts mem1 mem2 (lc1.(Local.coh) loc) (lc2.(Local.coh) loc))
-    (VRN: sim_view ts mem1 mem2 lc1.(Local.vrn) lc2.(Local.vrn))
-    (VWN: sim_view ts mem1 mem2 lc1.(Local.vwn) lc2.(Local.vwn))
-    (VRO: sim_view ts mem1 mem2 lc1.(Local.vro) lc2.(Local.vro))
-    (VWO: sim_view ts mem1 mem2 lc1.(Local.vwo) lc2.(Local.vwo))
-    (VCAP: sim_view ts mem1 mem2 lc1.(Local.vcap) lc2.(Local.vcap))
-    (VREL: sim_view ts mem1 mem2 lc1.(Local.vrel) lc2.(Local.vrel))
+    (COH: forall loc, sim_view ts (lc1.(Local.coh) loc) (lc2.(Local.coh) loc))
+    (VRN: sim_view ts lc1.(Local.vrn) lc2.(Local.vrn))
+    (VWN: sim_view ts lc1.(Local.vwn) lc2.(Local.vwn))
+    (VRO: sim_view ts lc1.(Local.vro) lc2.(Local.vro))
+    (VWO: sim_view ts lc1.(Local.vwo) lc2.(Local.vwo))
+    (VCAP: sim_view ts lc1.(Local.vcap) lc2.(Local.vcap))
+    (VREL: sim_view ts lc1.(Local.vrel) lc2.(Local.vrel))
     (FWDBANK: forall loc, sim_fwdbank ts mem1 mem2 loc (lc1.(Local.fwdbank) loc) (lc2.(Local.fwdbank) loc))
     (EXBANK: opt_rel (sim_exbank tid ts mem1 mem2) lc1.(Local.exbank) lc2.(Local.exbank))
     (PROMISES1: forall tsp (TSP: tsp <= ts), Promises.lookup tsp lc1.(Local.promises) = Promises.lookup tsp lc2.(Local.promises))
@@ -261,17 +260,17 @@ Hint Constructors sim_lc.
 
 Inductive sim_eu (tid:Id.t) (ts:Time.t) (eu1 eu2:ExecUnit.t (A:=unit)): Prop :=
 | sim_eu_intro
-    (STATE: sim_state ts eu1.(ExecUnit.mem) eu2.(ExecUnit.mem) eu1.(ExecUnit.state) eu2.(ExecUnit.state))
+    (STATE: sim_state ts eu1.(ExecUnit.state) eu2.(ExecUnit.state))
     (LOCAL: sim_lc tid ts eu1.(ExecUnit.mem) eu2.(ExecUnit.mem) eu1.(ExecUnit.local) eu2.(ExecUnit.local))
     (MEM: sim_mem tid ts eu1.(ExecUnit.mem) eu2.(ExecUnit.mem))
 .
 Hint Constructors sim_eu.
 
 Lemma sim_time_join
-      ts mem1 mem2 l1 l2 r1 r2
-      (VIEW1: sim_time ts mem1 mem2 l1 r1)
-      (VIEW2: sim_time ts mem1 mem2 l2 r2):
-  sim_time ts mem1 mem2 (join l1 l2) (join r1 r2).
+      ts l1 l2 r1 r2
+      (VIEW1: sim_time ts l1 r1)
+      (VIEW2: sim_time ts l2 r2):
+  sim_time ts (join l1 l2) (join r1 r2).
 Proof.
   inv VIEW1. inv VIEW2. econs.
   i. rewrite TS, TS0; ss.
@@ -280,8 +279,8 @@ Proof.
 Qed.
 
 Lemma sim_time_eq
-      ts mem1 mem2 v1 v2
-      (SIM: sim_time ts mem1 mem2 v1 v2)
+      ts v1 v2
+      (SIM: sim_time ts v1 v2)
       (V2: v2 <= ts):
   v1 = v2.
 Proof.
@@ -289,34 +288,32 @@ Proof.
 Qed.
 
 Lemma sim_val_const
-      ts mem1 mem2 c:
-  sim_val ts mem1 mem2 (ValA.mk _ c bot) (ValA.mk _ c bot).
+      ts c:
+  sim_val ts (ValA.mk _ c bot) (ValA.mk _ c bot).
 Proof.
   econs; splits; ss; try apply bot_spec.
 Qed.
 
 Lemma sim_view_bot
-      ts mem1 mem2:
-  sim_view ts mem1 mem2 bot bot.
+      ts:
+  sim_view ts bot bot.
 Proof.
   econs; splits; ss; try apply bot_spec.
 Qed.
 
 Lemma sim_view_const
-      ts mem1 mem2 c
-      (C1: c <= ts)
-      (C2: c <= length mem1)
-      (C3: c <= length mem2):
-  sim_view ts mem1 mem2 (View.mk c bot) (View.mk c bot).
+      ts c
+      (C1: c <= ts):
+  sim_view ts (View.mk c bot) (View.mk c bot).
 Proof.
   econs; ss.
 Qed.
 
 Lemma sim_view_join
-      ts mem1 mem2 l1 l2 r1 r2
-      (VIEW1: sim_view ts mem1 mem2 l1 r1)
-      (VIEW2: sim_view ts mem1 mem2 l2 r2):
-  sim_view ts mem1 mem2 (join l1 l2) (join r1 r2).
+      ts l1 l2 r1 r2
+      (VIEW1: sim_view ts l1 r1)
+      (VIEW2: sim_view ts l2 r2):
+  sim_view ts (join l1 l2) (join r1 r2).
 Proof.
   destruct l1 as [lt1 lv1].
   destruct l2 as [lt2 lv2].
@@ -329,33 +326,33 @@ Proof.
 Qed.
 
 Lemma sim_view_ifc
-      ts mem1 mem2 c l1 r1
-      (VIEW1: sim_view ts mem1 mem2 l1 r1):
-  sim_view ts mem1 mem2 (ifc c l1) (ifc c r1).
+      ts c l1 r1
+      (VIEW1: sim_view ts l1 r1):
+  sim_view ts (ifc c l1) (ifc c r1).
 Proof.
   destruct c; ss.
 Qed.
 
 Lemma sim_view_eq
-      ts mem1 mem2 v1 v2
-      (SIM: sim_view ts mem1 mem2 v1 v2)
+      ts v1 v2
+      (SIM: sim_view ts v1 v2)
       (V2: v2.(View.ts) <= ts):
   v1 = v2.
 Proof.
   apply SIM. ss.
 Qed.
 
-Lemma sim_val_view ts mem1 mem2 v1 v2
-      (VAL: sim_val ts mem1 mem2 v1 v2):
-  sim_view ts mem1 mem2 v1.(ValA.annot) v2.(ValA.annot).
+Lemma sim_val_view ts v1 v2
+      (VAL: sim_val ts v1 v2):
+  sim_view ts v1.(ValA.annot) v2.(ValA.annot).
 Proof.
   inv VAL. econs; ss. i. rewrite TS; ss.
 Qed.
 
 Lemma sim_rmap_expr
-      ts mem1 mem2 rmap1 rmap2 e
-      (RMAP: sim_rmap ts mem1 mem2 rmap1 rmap2):
-  sim_val ts mem1 mem2 (sem_expr rmap1 e) (sem_expr rmap2 e).
+      ts rmap1 rmap2 e
+      (RMAP: sim_rmap ts rmap1 rmap2):
+  sim_val ts (sem_expr rmap1 e) (sem_expr rmap2 e).
 Proof.
   induction e; s.
   - apply sim_val_const.
@@ -369,10 +366,10 @@ Proof.
 Qed.
 
 Lemma sim_rmap_add
-      ts mem1 mem2 rmap1 rmap2 v1 v2 r
-      (RMAP: sim_rmap ts mem1 mem2 rmap1 rmap2)
-      (VAL: sim_val ts mem1 mem2 v1 v2):
-  sim_rmap ts mem1 mem2 (RMap.add r v1 rmap1) (RMap.add r v2 rmap2).
+      ts rmap1 rmap2 v1 v2 r
+      (RMAP: sim_rmap ts rmap1 rmap2)
+      (VAL: sim_val ts v1 v2):
+  sim_rmap ts (RMap.add r v1 rmap1) (RMap.add r v2 rmap2).
 Proof.
   inv RMAP. econs. ii. unfold RMap.add. rewrite ? IdMap.add_spec.
   condtac; ss. inversion e. subst. econs. ss.
@@ -405,9 +402,9 @@ Proof.
 Qed.
 
 Lemma sim_view_val
-      ts mem1 mem2 c v1 v2
-      (SIM: sim_view ts mem1 mem2 v1 v2):
-  sim_val ts mem1 mem2 (ValA.mk _ c v1) (ValA.mk _ c v2).
+      ts c v1 v2
+      (SIM: sim_view ts v1 v2):
+  sim_val ts (ValA.mk _ c v1) (ValA.mk _ c v2).
 Proof.
   inv SIM. econs; ss. i. rewrite TS; ss.
 Qed.
@@ -429,7 +426,54 @@ Proof.
   destruct eu2' as [[stmts2' rmap2'] lc2' mem2'].
   inv SIM. inv STATE. ss. subst. inv STEP; cycle 1.
   { (* write step *)
-    admit.
+    inv STEP0. ss. inv STATE. inv PROMISE. inv FULFILL. ss.
+    eexists (ExecUnit.mk _ _ _). esplits.
+    - econs 2. econs; ss.
+      + econs; ss.
+      + econs; ss.
+        * inv WF1. ss. inv LOCAL0. inv WRITABLE. ss. econs; ss.
+          { eapply le_lt_trans; [|ss]. apply COH. }
+          { eapply le_lt_trans; [|ss]. s. admit. (* easy *) }
+          { intro X. specialize (EX X). des. inv LOCAL. inv EXBANK0; [congr|].
+            rewrite TSX in H. inv H. esplits; eauto.
+            destruct a, eb. ss. i. subst. inv REL. ss.
+            admit. (* ? *)
+          }
+        * unfold Memory.get_msg. s. rewrite nth_error_app2, Nat.sub_diag; ss.
+        * rewrite Promises.set_o. condtac; ss. congr.
+    - inv MEM2. inv WRITABLE. ss.
+      exploit sim_rmap_expr; eauto. i. inv x1. rewrite TS in *; cycle 1.
+      { rewrite <- VCAP. apply join_r. }
+      econs; ss.
+      + econs; ss. apply sim_rmap_add; ss. econs; ss.
+        unfold ifc. condtac; ss. intro Y. clear -Y MEM.
+        inv MEM. rewrite app_length in Y. lia.
+      + inv LOCAL. econs; ss.
+        * i. rewrite ? fun_add_spec. condtac; ss. admit. (* above *)
+        * apply sim_view_join; ss. admit. (* above *)
+        * apply sim_view_join; ss.
+        * apply sim_view_join; ss. unfold ifc. condtac; ss. admit. (* above *)
+        * i. rewrite ? fun_add_spec. condtac; ss.
+          { econs 2; ss.
+            - admit. (* ? *)
+            - admit. (* ? *)
+          }
+          { admit. (* ? *) }
+        * destruct ex; ss. inv EXBANK; econs; ss. inv REL. econs; ss.
+          admit. (* ? *)
+        * i. rewrite ? Promises.unset_o, ? Promises.set_o. condtac.
+          { inversion e. subst. admit. (* above *) }
+          condtac.
+          { inversion e. subst. admit. (* above *) }
+          apply PROMISES1. ss.
+        * i. rewrite Promises.unset_o, Promises.set_o. condtac; ss. eauto.
+      + inv MEM. ss. econs.
+        * ss.
+        * rewrite <- app_assoc. ss.
+        * rewrite <- app_assoc. ss.
+        * apply Forall_forall. i. apply in_app_iff in H. des.
+          { eapply Forall_forall in MEM1'; eauto. }
+          { inv H; ss. }
   }
   { (* state step *)
     inv STEP0. inv STEP. ss. subst. inv STATE; inv LOCAL0; inv EVENT.
@@ -457,91 +501,10 @@ Proof.
       exploit TS.
       { rewrite <- VCAP, <- join_r. ss. }
       intro ELOC. rewrite ELOC in *. clear TS.
-      destruct (ts0 == (lc2.(Local.fwdbank) (ValA.val (sem_expr rmap2 eloc))).(FwdItem.ts)).
-      { (* Case 1: Tgt read from fwdbank. Src reads from fwdbank, too. *)
-        inv e. inv LOCAL. exploit sim_fwd_view1; eauto.
-        { apply WF1. }
-        { apply WF2. }
-        intro FWDVIEW.
-        eexists (ExecUnit.mk _ _ _). esplits.
-        - econs 1. econs. econs; ss.
-          + econs; ss.
-          + rewrite ELOC in *.
-            econs 2; eauto. econs; ss; cycle 2.
-            * 
-              Lemma read_app1_inv ts loc val mem1 mem2
-                    (TS: ts <= length mem1)
-                    (READ: Memory.read loc ts (mem1 ++ mem2) = Some val):
-                Memory.read loc ts mem1 = Some val.
-              Proof.
-                revert READ. unfold Memory.read. destruct ts; ss.
-                destruct (nth_error (mem1 ++ mem2) ts) eqn:NTH; ss.
-                rewrite nth_error_app1 in NTH; ss. rewrite NTH. ss.
-              Qed.
-              Lemma sim_fwdbank_read
-                    ts mem1 mem2 loc fwd1 fwd2
-                    (SIM: sim_fwdbank ts mem1 mem2 loc fwd1 fwd2):
-                Memory.read loc fwd1.(FwdItem.ts) mem1 = Memory.read loc fwd2.(FwdItem.ts) mem2.
-              Proof.
-                inv SIM; ss.
-              Qed.
-
-              erewrite sim_fwdbank_read; eauto.
-            * destruct (FWDBANK (ValA.val (sem_expr rmap2 eloc))).
-              { rewrite FWD. admit.
-                (* 1. if lc2.coh <= ts, then obvious. *)
-                (* 2. if lc2.coh > ts, then there should be no msg of > ts in src. *)
-              }
-              { eapply Memory.latest_mon2; eauto. inv WF1. ss. inv LOCAL. apply COH1. }
-            * admit. (* external, similar *)
-        - econs; ss.
-          + econs; ss. apply sim_rmap_add; ss. apply sim_view_val.
-            rewrite POST. eauto 10 using sim_view_join, sim_view_ifc, sim_view_bot.
-          + econs; ss; try by rewrite ? POST; eauto 10 using sim_view_join, sim_view_ifc, sim_view_bot.
-            * i. rewrite ? fun_add_spec. condtac; ss.
-              rewrite ? POST; eauto 10 using sim_view_join, sim_view_ifc, sim_view_bot.
-            * destruct ex0; ss. econs. econs; ss.
-              { destruct (FWDBANK (ValA.val (sem_expr rmap2 eloc))).
-                - admit. (* easy *)
-                - ii. des. eapply LATEST0; eauto. rewrite TS2, BELOW.
-                  inv MEM. rewrite app_length. clear. lia.
-              }
-              { rewrite POST. eauto 10 using sim_view_join, sim_view_ifc, sim_view_bot. }
-      }
-
-      (* Now tgt didn't read from fwdbank. *)
-      assert (FWD_ABOVE: FwdItem.ts (Local.fwdbank lc2 (ValA.val (sem_expr rmap2 eloc))) < ts0).
-      { admit. }
 
       (* Case analysis on [tgt's post-view <= ts]. *)
-      destruct (le_lt_dec post.(View.ts) ts).
-      { (* Case 2: Tgt didn't read from fwdbank, and tgt's post-view <= ts. Src reads the same msg. *)
-        rename l into POST_BELOW. inv LOCAL.
-        exploit sim_fwd_view2; eauto.
-        { apply WF1. }
-        { apply WF2. }
-        intro FWDVIEW.
-        assert (BELOW: ts0 <= ts).
-        { admit. }
-        eexists (ExecUnit.mk _ _ _). esplits.
-        - econs 1. econs. econs; ss.
-          + econs; ss.
-          + rewrite ELOC in *.
-            econs 2; eauto. econs; ss; cycle 2.
-            * erewrite sim_mem_read; eauto.
-            * admit. (* coh, similar *)
-            * admit. (* external, similar *)
-        - econs; ss.
-          + econs; ss. apply sim_rmap_add; ss. apply sim_view_val.
-            rewrite POST. eauto 10 using sim_view_join, sim_view_ifc, sim_view_bot.
-          + econs; ss; try by rewrite ? POST; eauto 10 using sim_view_join, sim_view_ifc, sim_view_bot.
-            * i. rewrite ? fun_add_spec. condtac; ss.
-              rewrite ? POST; eauto 10 using sim_view_join, sim_view_ifc, sim_view_bot.
-            * destruct ex0; ss. econs. econs; ss.
-              { admit. (* easy *) }
-              { rewrite POST. eauto 10 using sim_view_join, sim_view_ifc, sim_view_bot. }
-      }
-      { (* Case 3: Tgt didn't read from fwdbank, and tgt's post-view > ts. Src reads the latest msg. *)
+      destruct (le_lt_dec post.(View.ts) ts); cycle 1.
+      { (* Case 3: Tgt's post-view > ts. Src reads the latest msg. *)
         rename l into POST_ABOVE. inv LOCAL.
         exploit Memory.latest_ts_spec; eauto. i. des.
         eexists (ExecUnit.mk _ _ _). esplits.
@@ -570,6 +533,72 @@ Proof.
             * destruct ex0; ss. econs. econs; ss.
               { admit. (* easy *) }
               { admit. (* POST_ABOVE *) }
+      }
+
+      (* Tgt's post-view <= ts. *)
+      rename l into POST_BELOW.
+      (* Now case analysis on whether tgt read from fwdbank. *)
+      destruct (ts0 == (lc2.(Local.fwdbank) (ValA.val (sem_expr rmap2 eloc))).(FwdItem.ts)).
+      { (* Case 2: Tgt read from fwdbank. Src reads from fwdbank, too. *)
+        inv e. inv LOCAL. exploit sim_fwd_view1; eauto.
+        { apply WF1. }
+        { apply WF2. }
+        intro FWDVIEW.
+        eexists (ExecUnit.mk _ _ _). esplits.
+        - econs 1. econs. econs; ss.
+          + econs; ss.
+          + rewrite ELOC in *.
+            econs 2; eauto. econs; ss; cycle 2.
+            * destruct (FWDBANK (ValA.val (sem_expr rmap2 eloc))).
+              { rewrite READ. eauto. }
+              { admit. (* contradiction from POST_BELOW and ABOVE *) }
+            * destruct (FWDBANK (ValA.val (sem_expr rmap2 eloc))).
+              { rewrite FWD. admit.
+                (* 1. if lc2.coh <= ts, then obvious. *)
+                (* 2. if lc2.coh > ts, then there should be no msg of > ts in src. *)
+              }
+              { eapply Memory.latest_mon2; eauto. inv WF1. ss. inv LOCAL. apply COH1. }
+            * admit. (* external, similar *)
+        - econs; ss.
+          + econs; ss. apply sim_rmap_add; ss. apply sim_view_val.
+            rewrite POST. eauto 10 using sim_view_join, sim_view_ifc, sim_view_bot.
+          + econs; ss; try by rewrite ? POST; eauto 10 using sim_view_join, sim_view_ifc, sim_view_bot.
+            * i. rewrite ? fun_add_spec. condtac; ss.
+              rewrite ? POST; eauto 10 using sim_view_join, sim_view_ifc, sim_view_bot.
+            * destruct ex0; ss. econs. econs; ss.
+              { destruct (FWDBANK (ValA.val (sem_expr rmap2 eloc))).
+                - admit. (* easy *)
+                - ii. des. eapply LATEST0; eauto. rewrite TS2, BELOW.
+                  inv MEM. rewrite app_length. clear. lia.
+              }
+              { rewrite POST. eauto 10 using sim_view_join, sim_view_ifc, sim_view_bot. }
+      }
+      { (* Case 3: Tgt didn't read from fwdbank. Src reads the same msg. *)
+        assert (FWD_ABOVE: FwdItem.ts (Local.fwdbank lc2 (ValA.val (sem_expr rmap2 eloc))) < ts0).
+        { admit. }
+        inv LOCAL. exploit sim_fwd_view2; eauto.
+        { apply WF1. }
+        { apply WF2. }
+        intro FWDVIEW.
+        assert (BELOW: ts0 <= ts).
+        { admit. }
+        eexists (ExecUnit.mk _ _ _). esplits.
+        - econs 1. econs. econs; ss.
+          + econs; ss.
+          + rewrite ELOC in *.
+            econs 2; eauto. econs; ss; cycle 2.
+            * erewrite sim_mem_read; eauto.
+            * admit. (* coh, similar *)
+            * admit. (* external, similar *)
+        - econs; ss.
+          + econs; ss. apply sim_rmap_add; ss. apply sim_view_val.
+            rewrite POST. eauto 10 using sim_view_join, sim_view_ifc, sim_view_bot.
+          + econs; ss; try by rewrite ? POST; eauto 10 using sim_view_join, sim_view_ifc, sim_view_bot.
+            * i. rewrite ? fun_add_spec. condtac; ss.
+              rewrite ? POST; eauto 10 using sim_view_join, sim_view_ifc, sim_view_bot.
+            * destruct ex0; ss. econs. econs; ss.
+              { admit. (* easy *) }
+              { rewrite POST. eauto 10 using sim_view_join, sim_view_ifc, sim_view_bot. }
       }
     - (* fulfill *)
       inv STEP.
@@ -788,32 +817,16 @@ Proof.
   inv CERTIFY. econs; [|by eauto]. econs; eauto.
 Qed.
 
-(* TODO: move *)
-Lemma sim_view_app2
-      ts mem1 mem2 mem2' v1 v2
-      (SIM: sim_view ts mem1 mem2 v1 v2):
-  sim_view ts mem1 (mem2 ++ mem2') v1 v2.
-Proof.
-  inv SIM. econs; ss.
-Qed.
 Lemma sim_view_refl
-      ts mem v
-      (VIEW: v.(View.ts) <= length mem):
-  sim_view ts mem mem v v.
+      ts v:
+  sim_view ts v v.
 Proof.
   econs; ss.
 Qed.
-Lemma sim_time_app2
-      ts mem1 mem2 mem2' t1 t2
-      (SIM: sim_time ts mem1 mem2 t1 t2):
-  sim_time ts mem1 (mem2 ++ mem2') t1 t2.
-Proof.
-  inv SIM. econs; ss.
-Qed.
+
 Lemma sim_time_refl
-      ts mem t
-      (TIME: t <= length mem):
-  sim_time ts mem mem t t.
+      ts t:
+  sim_time ts t t.
 Proof.
   econs; ss.
 Qed.
